\def\arraystretch{0.8}
\begin{array}{c c}
\beta\text{ Reduction}&\\ 
     \hline \\
  (\lambda x .M) N \rightarrow_\beta M[x := N]& \text{basis}\\ \\
  \cfrac{B\rightarrow_\beta B'}{\lambda x :A.\ B \rightarrow_\beta \lambda x :A.\ B'}  & \\ \\
  \cfrac{A\rightarrow_\beta A'}{\lambda x :A.\ B \rightarrow_\beta \lambda x :A'.\ B}  & \\ \\
  \cfrac{B\rightarrow_\beta B'}{\Pi x :A.\ B \rightarrow_\beta \Pi x :A.\ B'}  & \\ \\
  \cfrac{A\rightarrow_\beta A'}{\Pi x :A.\ B \rightarrow_\beta \Pi x :A'.\ B}  & \\ \\
  \text{Beta Reduction takes a } & \text{} \\ 
  \text{reducible expression, and} &  \\ 
  \text{converts it into a contraction} &  \\ 
  \text{as seen in the basis rule.} &  \\ \\
  \text{Beta Reduction is shown by} & \rightarrow_\beta \\ 
  \text{Beta Conversion is shown by} & =_\beta \\ 
\end{array}